src/Pred.v
@@ -14,12 +14,13 @@ Set Implicit Arguments.
 
 Section GenPredDef.
 
-Variable len : nat.
+Variable AT : Type.
+Variable AEQ : DecEq AT.
 Variable V : Type.
 
-Definition pred := @mem len V -> Prop.
+Definition pred := @mem AT AEQ V -> Prop.
 
-Definition ptsto (a : word len) (v : V) : pred :=
+Definition ptsto (a : AT) (v : V) : pred :=
   fun m => m a = Some v /\ forall a', a <> a' -> m a' = None.
 
 Definition impl (p q : pred) : pred :=
@@ -56,10 +57,10 @@ Definition pimpl (p q : pred) := forall m, p m -> q m.
 
 Definition piff (p q : pred) : Prop := (pimpl p q) /\ (pimpl q p).
 
-Definition mem_disjoint (m1 m2 : @mem len V) :=
+Definition mem_disjoint (m1 m2 : @mem AT AEQ V) :=
   ~ exists a (v1 v2 : V), m1 a = Some v1 /\ m2 a = Some v2.
 
-Definition mem_union (m1 m2 : @mem len V) : mem := fun a =>
+Definition mem_union (m1 m2 : @mem AT AEQ V) : (@mem AT AEQ V) := fun a =>
   match m1 a with
   | Some v => Some v
   | None => m2 a
@@ -68,18 +69,18 @@ Definition mem_union (m1 m2 : @mem len V) : mem := fun a =>
 Definition sep_star_impl (p1: pred) (p2: pred) : pred :=
   fun m => exists m1 m2, m = mem_union m1 m2 /\ mem_disjoint m1 m2 /\ p1 m1 /\ p2 m2.
 
-Definition indomain (a: word len) (m: mem) :=
+Definition indomain (a: AT) (m: @mem AT AEQ V) :=
   exists (v:V), m a = Some v.
 
 End GenPredDef.
 
-Arguments pred {len V}.
-Arguments emp {len V} _.
-Arguments any {len V} _.
-Arguments pimpl {len V} _ _.
-Arguments piff {len V} _ _.
-Arguments sep_star_impl {len V} _ _ _.
-Arguments indomain {len V} _ _.
+Arguments pred {AT AEQ V}.
+Arguments emp {AT AEQ V} _.
+Arguments any {AT AEQ V} _.
+Arguments pimpl {AT AEQ V} _ _.
+Arguments piff {AT AEQ V} _ _.
+Arguments sep_star_impl {AT AEQ V} _ _ _.
+Arguments indomain {AT AEQ V} _ _.
 
 Hint Unfold pimpl.
 Hint Unfold piff.
@@ -102,7 +103,7 @@ Notation "p <=p=> q" := (piff p%pred q%pred) (at level 90).
 
 
 Module Type SEP_STAR.
-  Parameter sep_star : forall {len:nat} {V:Type}, @pred len V -> @pred len V -> @pred len V.
+  Parameter sep_star : forall {AT:Type} {AEQ:DecEq AT} {V:Type}, @pred AT AEQ V -> @pred AT AEQ V -> @pred AT AEQ V.
   Axiom sep_star_is : @sep_star = @sep_star_impl.
 End SEP_STAR.
 
@@ -114,7 +115,7 @@ End Sep_Star.
 
 Definition sep_star := @Sep_Star.sep_star.
 Definition sep_star_is := Sep_Star.sep_star_is.
-Arguments sep_star {len V} _ _ _.
+Arguments sep_star {AT AEQ V} _ _ _.
 Infix "*" := sep_star : pred_scope.
 
 
@@ -126,7 +127,7 @@ Notation "a |~> v" := (exists old, a |-> ((v, old) : valuset))%pred (at level 35
 
 
 (* if [p] was true before a crash, then [crash_xform p] is true after a crash *)
-Definition crash_xform (p : pred) : @pred addrlen valuset :=
+Definition crash_xform {AT : Type} {AEQ : DecEq AT} (p : pred) : @pred AT AEQ valuset :=
   fun m => exists m', p m' /\ possible_crash m' m.
 
 
@@ -146,10 +147,11 @@ Ltac unfold_sep_star :=
 
 Section GenPredThm.
 
-Variable len : nat.
+Variable AT : Type.
+Variable AEQ : DecEq AT.
 Variable V : Type.
 
-Theorem pimpl_refl : forall (p : @pred len V), p =p=> p.
+Theorem pimpl_refl : forall (p : @pred AT AEQ V), p =p=> p.
 Proof.
   pred.
 Qed.
@@ -157,14 +159,14 @@ Qed.
 Hint Resolve pimpl_refl.
 
 Theorem mem_disjoint_comm:
-  forall (m1 m2 : @mem len V),
+  forall (m1 m2 : @mem AT AEQ V),
   mem_disjoint m1 m2 <-> mem_disjoint m2 m1.
 Proof.
   split; unfold mem_disjoint, not; intros; repeat deex; eauto 10.
 Qed.
 
 Theorem mem_disjoint_assoc_1:
-  forall (m1 m2 m3 : @mem len V),
+  forall (m1 m2 m3 : @mem AT AEQ V),
   mem_disjoint m1 m2 ->
   mem_disjoint (mem_union m1 m2) m3 ->
   mem_disjoint m1 (mem_union m2 m3).
@@ -177,7 +179,7 @@ Proof.
 Qed.
 
 Theorem mem_disjoint_assoc_2:
-  forall (m1 m2 m3 : @mem len V),
+  forall (m1 m2 m3 : @mem AT AEQ V),
   mem_disjoint m2 m3 ->
   mem_disjoint m1 (mem_union m2 m3) ->
   mem_disjoint (mem_union m1 m2) m3.
@@ -191,7 +193,7 @@ Proof.
 Qed.
 
 Theorem mem_disjoint_union:
-  forall (m1 m2 m3 : @mem len V),
+  forall (m1 m2 m3 : @mem AT AEQ V),
   mem_disjoint (mem_union m1 m2) m3 ->
   mem_disjoint m2 m3.
 Proof.
@@ -200,17 +202,17 @@ Proof.
 Qed.
 
 Theorem mem_disjoint_upd:
-  forall m1 m2 (a : word len) (v:V) v0,
+  forall (m1 m2 : @mem AT AEQ V) a v v0,
   m1 a = Some v0 ->
   mem_disjoint m1 m2 ->
   mem_disjoint (upd m1 a v) m2.
 Proof.
   unfold mem_disjoint, upd, not; intros; repeat deex;
-    destruct (weq x a); subst; eauto 10.
+    destruct (AEQ x a); subst; eauto 10.
 Qed.
 
 Theorem mem_union_comm:
-  forall (m1 m2 : @mem len V),
+  forall (m1 m2 : @mem AT AEQ V),
   mem_disjoint m1 m2 ->
   mem_union m1 m2 = mem_union m2 m1.
 Proof.
@@ -219,7 +221,7 @@ Proof.
 Qed.
 
 Theorem mem_union_addr:
-  forall m1 m2 (a : word len) (v:V),
+  forall (m1 m2 : @mem AT AEQ V) a v,
   mem_disjoint m1 m2 ->
   m1 a = Some v ->
   mem_union m1 m2 a = Some v.
@@ -228,16 +230,16 @@ Proof.
 Qed.
 
 Theorem mem_union_upd:
-  forall m1 m2 (a : word len) (v:V) v0,
+  forall (m1 m2 : @mem AT AEQ V) a v v0,
   m1 a = Some v0 ->
   mem_union (upd m1 a v) m2 = upd (mem_union m1 m2) a v.
 Proof.
   unfold mem_union, upd; intros; apply functional_extensionality; intros.
-  destruct (weq x a); eauto.
+  destruct (AEQ x a); eauto.
 Qed.
 
 Theorem mem_union_assoc:
-  forall (m1 m2 m3 : @mem len V),
+  forall (m1 m2 m3 : @mem AT AEQ V),
   mem_disjoint m1 m2 ->
   mem_disjoint (mem_union m1 m2) m3 ->
   mem_union (mem_union m1 m2) m3 = mem_union m1 (mem_union m2 m3).
@@ -247,7 +249,7 @@ Proof.
 Qed.
 
 Theorem sep_star_comm1:
-  forall (p1 p2 : @pred len V),
+  forall (p1 p2 : @pred AT AEQ V),
   (p1 * p2 =p=> p2 * p1)%pred.
 Proof.
   unfold pimpl; unfold_sep_star; pred.
@@ -255,14 +257,14 @@ Proof.
 Qed.
 
 Theorem sep_star_comm:
-  forall (p1 p2 : @pred len V),
+  forall (p1 p2 : @pred AT AEQ V),
   (p1 * p2 <=p=> p2 * p1)%pred.
 Proof.
   unfold piff; split; apply sep_star_comm1.
 Qed.
 
 Theorem sep_star_assoc_1:
-  forall (p1 p2 p3 : @pred len V),
+  forall (p1 p2 p3 : @pred AT AEQ V),
   (p1 * p2 * p3 =p=> p1 * (p2 * p3))%pred.
 Proof.
   unfold pimpl; unfold_sep_star; pred.
@@ -274,7 +276,7 @@ Proof.
 Qed.
 
 Theorem sep_star_assoc_2:
-  forall (p1 p2 p3 : @pred len V),
+  forall (p1 p2 p3 : @pred AT AEQ V),
   (p1 * (p2 * p3) =p=> p1 * p2 * p3)%pred.
 Proof.
   unfold pimpl; unfold_sep_star; pred.
@@ -291,7 +293,7 @@ Proof.
 Qed.
 
 Theorem sep_star_assoc:
-  forall (p1 p2 p3 : @pred len V),
+  forall (p1 p2 p3 : @pred AT AEQ V),
   (p1 * p2 * p3 <=p=> p1 * (p2 * p3))%pred.
 Proof.
   split; [ apply sep_star_assoc_1 | apply sep_star_assoc_2 ].
@@ -303,7 +305,7 @@ Local Hint Extern 1 =>
   end.
 
 Lemma pimpl_exists_l:
-  forall T p (q : @pred len V),
+  forall T p (q : @pred AT AEQ V),
   (forall x:T, p x =p=> q) ->
   (exists x:T, p x) =p=> q.
 Proof.
@@ -311,7 +313,7 @@ Proof.
 Qed.
 
 Lemma pimpl_exists_r:
-  forall T (p : @pred len V) q,
+  forall T (p : @pred AT AEQ V) q,
   (exists x:T, p =p=> q x) ->
   (p =p=> exists x:T, q x).
 Proof.
@@ -319,7 +321,7 @@ Proof.
 Qed.
 
 Lemma pimpl_exists_l_star:
-  forall T p (q : @pred len V) r,
+  forall T p (q : @pred AT AEQ V) r,
   ((exists x:T, p x * r) =p=> q) ->
   (exists x:T, p x) * r =p=> q.
 Proof.
@@ -331,7 +333,7 @@ Proof.
 Qed.
 
 Lemma pimpl_exists_r_star:
-  forall T p (q : @pred len V),
+  forall T p (q : @pred AT AEQ V),
   (exists x:T, p x * q) =p=> ((exists x:T, p x) * q).
 Proof.
   unfold pimpl, exis; unfold_sep_star; intros.
@@ -341,7 +343,7 @@ Proof.
 Qed.
 
 Lemma pimpl_exists_l_and:
-  forall T p (q : @pred len V) r,
+  forall T p (q : @pred AT AEQ V) r,
   ((exists x:T, p x /\ r) =p=> q) ->
   (exists x:T, p x) /\ r =p=> q.
 Proof.
@@ -349,7 +351,7 @@ Proof.
 Qed.
 
 Lemma pimpl_trans:
-  forall (a b c : @pred len V),
+  forall (a b c : @pred AT AEQ V),
   (a =p=> b) ->
   (b =p=> c) ->
   (a =p=> c).
@@ -358,7 +360,7 @@ Proof.
 Qed.
 
 Lemma pimpl_trans2:
-  forall (a b c : @pred len V),
+  forall (a b c : @pred AT AEQ V),
   (b =p=> c) ->
   (a =p=> b) ->
   (a =p=> c).
@@ -367,7 +369,7 @@ Proof.
 Qed.
 
 Lemma piff_trans:
-  forall (a b c : @pred len V),
+  forall (a b c : @pred AT AEQ V),
   (a <=p=> b) ->
   (b <=p=> c) ->
   (a <=p=> c).
@@ -376,7 +378,7 @@ Proof.
 Qed.
 
 Lemma piff_comm:
-  forall (a b : @pred len V),
+  forall (a b : @pred AT AEQ V),
   (a <=p=> b) ->
   (b <=p=> a).
 Proof.
@@ -384,14 +386,14 @@ Proof.
 Qed.
 
 Lemma piff_refl:
-  forall (a : @pred len V),
+  forall (a : @pred AT AEQ V),
   (a <=p=> a).
 Proof.
   unfold piff; intuition.
 Qed.
 
 Lemma pimpl_apply:
-  forall (p q:@pred len V) m,
+  forall (p q:@pred AT AEQ V) m,
   (p =p=> q) ->
   p m ->
   q m.
@@ -400,7 +402,7 @@ Proof.
 Qed.
 
 Lemma piff_apply:
-  forall (p q:@pred len V) m,
+  forall (p q:@pred AT AEQ V) m,
   (p <=p=> q) ->
   q m ->
   p m.
@@ -409,21 +411,21 @@ Proof.
 Qed.
 
 Lemma pimpl_fun_l:
-  forall (p:@pred len V),
+  forall (p:@pred AT AEQ V),
   (fun m => p m) =p=> p.
 Proof.
   firstorder.
 Qed.
 
 Lemma pimpl_fun_r:
-  forall (p:@pred len V),
+  forall (p:@pred AT AEQ V),
   p =p=> (fun m => p m).
 Proof.
   firstorder.
 Qed.
 
 Lemma pimpl_sep_star:
-  forall (a b c d : @pred len V),
+  forall (a b c d : @pred AT AEQ V),
   (a =p=> c) ->
   (b =p=> d) ->
   (a * b =p=> c * d).
@@ -435,7 +437,7 @@ Proof.
 Qed.
 
 Lemma pimpl_and:
-  forall (a b c d : @pred len V),
+  forall (a b c d : @pred AT AEQ V),
   (a =p=> c) ->
   (b =p=> d) ->
   (a /\ b =p=> c /\ d).
@@ -443,7 +445,7 @@ Proof.
   firstorder.
 Qed.
 
-Lemma pimpl_or : forall (p q p' q' : @pred len V),
+Lemma pimpl_or : forall (p q p' q' : @pred AT AEQ V),
   p =p=> p'
   -> q =p=> q'
   -> p \/ q =p=> p' \/ q'.
@@ -452,7 +454,7 @@ Proof.
 Qed.
 
 Lemma sep_star_lift_l:
-  forall (a: Prop) (b c: @pred len V),
+  forall (a: Prop) (b c: @pred AT AEQ V),
   (a -> (b =p=> c)) ->
   b * [[a]] =p=> c.
 Proof.
@@ -465,7 +467,7 @@ Proof.
 Qed.
 
 Lemma sep_star_lift_r':
-  forall (b: Prop) (a c: @pred len V),
+  forall (b: Prop) (a c: @pred AT AEQ V),
   (a =p=> [b] /\ c) ->
   (a =p=> [[b]] * c).
 Proof.
@@ -477,7 +479,7 @@ Proof.
 Qed.
 
 Lemma sep_star_lift_r:
-  forall (a b: @pred len V) (c: Prop),
+  forall (a b: @pred AT AEQ V) (c: Prop),
   (a =p=> b /\ [c]) ->
   (a =p=> b * [[c]]).
 Proof.
@@ -487,7 +489,7 @@ Proof.
   firstorder.
 Qed.
 
-Theorem sep_star_lift_apply : forall (a : Prop) (b : @pred len V) (m : mem),
+Theorem sep_star_lift_apply : forall (a : Prop) (b : @pred AT AEQ V) (m : mem),
   (b * [[a]])%pred m -> (b m /\ a).
 Proof.
   unfold lift_empty; unfold_sep_star; intros.
@@ -498,7 +500,7 @@ Proof.
   congruence.
 Qed.
 
-Lemma pimpl_star_emp: forall (p : @pred len V), p =p=> emp * p.
+Lemma pimpl_star_emp: forall (p : @pred AT AEQ V), p =p=> emp * p.
 Proof.
   unfold pimpl; unfold_sep_star; intros.
   repeat eexists; eauto.
@@ -506,7 +508,7 @@ Proof.
   unfold mem_disjoint; pred.
 Qed.
 
-Lemma star_emp_pimpl: forall (p : @pred len V), emp * p =p=> p.
+Lemma star_emp_pimpl: forall (p : @pred AT AEQ V), emp * p =p=> p.
 Proof.
   unfold pimpl; unfold_sep_star; intros.
   unfold emp in *; pred.
@@ -516,12 +518,12 @@ Proof.
   pred.
 Qed.
 
-Lemma emp_star: forall p, p <=p=> (@emp len V) * p.
+Lemma emp_star: forall p, p <=p=> (@emp AT AEQ V) * p.
 Proof.
   intros; split; [ apply pimpl_star_emp | apply star_emp_pimpl ].
 Qed.
 
-Lemma piff_star_r: forall (a b c : @pred len V),
+Lemma piff_star_r: forall (a b c : @pred AT AEQ V),
   (a <=p=> b) ->
   (a * c <=p=> b * c).
 Proof.
@@ -529,7 +531,7 @@ Proof.
     repeat deex; repeat eexists; eauto.
 Qed.
 
-Lemma piff_star_l: forall (a b c : @pred len V),
+Lemma piff_star_l: forall (a b c : @pred AT AEQ V),
   (a <=p=> b) ->
   (c * a <=p=> c * b).
 Proof.
@@ -538,7 +540,7 @@ Proof.
 Qed.
 
 Lemma piff_l :
-  forall (p p' q : @pred len V),
+  forall (p p' q : @pred AT AEQ V),
   (p <=p=> p')
   -> (p' =p=> q)
   -> (p =p=> q).
@@ -547,7 +549,7 @@ Proof.
 Qed.
 
 Lemma piff_r :
-  forall (p q q' : @pred len V),
+  forall (p q q' : @pred AT AEQ V),
   (q <=p=> q')
   -> (p =p=> q')
   -> (p =p=> q).
@@ -556,7 +558,7 @@ Proof.
 Qed.
 
 Lemma sep_star_lift2and:
-  forall (a : @pred len V) b,
+  forall (a : @pred AT AEQ V) b,
   (a * [[b]]) =p=> a /\ [b].
 Proof.
   unfold and, lift, lift_empty, pimpl; unfold_sep_star.
@@ -568,7 +570,7 @@ Proof.
 Qed.
 
 Lemma sep_star_and2lift:
-  forall (a : @pred len V) b,
+  forall (a : @pred AT AEQ V) b,
   (a /\ [b]) =p=> (a * [[b]]).
 Proof.
   unfold and, lift, lift_empty, pimpl; unfold_sep_star.
@@ -589,7 +591,7 @@ Proof.
 Qed.
 
 Lemma ptsto_valid:
-  forall (a : word len) (v : V) F m,
+  forall a v F (m : @mem AT AEQ V),
   (a |-> v * F)%pred m
   -> m a = Some v.
 Proof.
@@ -599,7 +601,7 @@ Proof.
 Qed.
 
 Lemma ptsto_valid':
-  forall (a : word len) (v : V) F m,
+  forall a v F (m : @mem AT AEQ V),
   (F * (a |-> v))%pred m
   -> m a = Some v.
 Proof.
@@ -611,80 +613,80 @@ Proof.
 Qed.
 
 
-Lemma ptsto_upd_disjoint: forall V (F : @pred len V) a v m,
+Lemma ptsto_upd_disjoint: forall V (F : @pred AT AEQ V) a v m,
   F m -> m a = None
   -> (F * a |-> v)%pred (upd m a v).
 Proof.
   unfold upd; unfold_sep_star; intros; repeat deex.
   exists m.
-  exists (fun a' => if weq a' a then Some v else None).
+  exists (fun a' => if AEQ a' a then Some v else None).
   split; [|split].
   - apply functional_extensionality; intro.
-    unfold mem_union; destruct (weq x a); subst; intuition.
+    unfold mem_union; destruct (AEQ x a); subst; intuition.
     rewrite H0; auto.
     destruct (m x); auto.
   - unfold mem_disjoint in *. intuition. repeat deex.
-    destruct (weq x a); subst; intuition; pred.
+    destruct (AEQ x a); subst; intuition; pred.
   - intuition; eauto.
     unfold ptsto; intuition.
-    destruct (weq a a); pred.
-    destruct (weq a' a); pred.
+    destruct (AEQ a a); pred.
+    destruct (AEQ a' a); pred.
 Qed.
 
 
 Lemma ptsto_upd:
-  forall (a : word len) (v v0 : V) F m,
+  forall a v v0 F (m : @mem AT AEQ V),
   (a |-> v0 * F)%pred m ->
   (a |-> v * F)%pred (upd m a v).
 Proof.
   unfold upd; unfold_sep_star; intros; repeat deex.
-  exists (fun a' => if weq a' a then Some v else None).
+  exists (fun a' => if AEQ a' a then Some v else None).
   exists x0.
   split; [|split].
   - apply functional_extensionality; intro.
-    unfold mem_union; destruct (weq x1 a); eauto.
+    unfold mem_union; destruct (AEQ x1 a); eauto.
     destruct H1; repeat deex.
     rewrite H1; auto.
   - unfold mem_disjoint in *. intuition. repeat deex.
     apply H.
     destruct H1; repeat deex.
     repeat eexists; eauto.
-    destruct (weq x1 a); subst; eauto.
+    destruct (AEQ x1 a); subst; eauto.
     pred.
   - intuition eauto.
     unfold ptsto; intuition.
-    destruct (weq a a); pred.
-    destruct (weq a' a); pred.
+    destruct (AEQ a a); pred.
+    destruct (AEQ a' a); pred.
 Qed.
 
 Lemma ptsto_upd_bwd:
-  forall (a b : word len) (v w : V) F m,
+  forall a b v w F (m : @mem AT AEQ V),
   a <> b ->
   (a |-> v * F)%pred (upd m b w) ->
   (a |-> v * any)%pred m.
 Proof.
   unfold upd, ptsto; unfold_sep_star; intros; repeat deex.
-  exists (fun a' => if weq a' a then Some v else None).
-  exists (fun a' => if weq a' b then m a' else x0 a').
+  exists (fun a' => if AEQ a' a then Some v else None).
+  exists (fun a' => if AEQ a' b then m a' else x0 a').
   split; [|split].
   - apply functional_extensionality; intros.
     unfold mem_union in *. pose proof (equal_f H1 x1); clear H1; simpl in *.
-    destruct (weq x1 a); subst.
-    + rewrite H3 in H2. destruct (weq a b); congruence.
+    destruct (AEQ x1 a); subst.
+    + rewrite H3 in H2. destruct (AEQ a b); congruence.
     + rewrite H5 in H2 by congruence.
-      destruct (weq x1 b); congruence.
+      destruct (AEQ x1 b); congruence.
   - unfold mem_disjoint in *. intuition. repeat deex.
     apply H0; clear H0.
-    destruct (weq x1 a); destruct (weq x1 b); subst; try congruence.
+    destruct (AEQ x1 a); destruct (AEQ x1 b); subst; try congruence.
     repeat eexists; eauto.
   - intuition eauto.
-    destruct (weq a a); congruence.
-    destruct (weq a' a); congruence.
+    destruct (AEQ a a); congruence.
+    destruct (AEQ a' a); congruence.
     firstorder.
 Qed.
 
 
-Lemma ptsto_eq : forall (p1 p2 : @pred len V) m a v1 v2,
+Lemma ptsto_eq : forall (p1 p2 : @pred AT AEQ V) m a v1 v2,
   p1 m -> p2 m ->
   (exists F, p1 =p=> a |-> v1 * F) ->
   (exists F, p2 =p=> a |-> v2 * F) ->
@@ -701,7 +703,7 @@ Proof.
 Qed.
 
 Lemma pimpl_and_split:
-  forall (a b c : @pred len V),
+  forall (a b c : @pred AT AEQ V),
   (a =p=> b)
   -> (a =p=> c)
   -> (a =p=> b /\ c).
@@ -709,7 +711,7 @@ Proof.
   firstorder.
 Qed.
 
-Lemma pimpl_and_lift: forall (a b: @pred len V) (c:Prop),
+Lemma pimpl_and_lift: forall (a b: @pred AT AEQ V) (c:Prop),
   (a =p=> b)
   -> c
   -> (a =p=> b /\ [c]).
@@ -717,7 +719,7 @@ Proof.
   firstorder.
 Qed.
 
-Lemma pimpl_or_l: forall (a b c: @pred len V),
+Lemma pimpl_or_l: forall (a b c: @pred AT AEQ V),
   (a =p=> c)
   -> (b =p=> c)
   -> (a \/ b =p=> c).
@@ -725,7 +727,7 @@ Proof.
   firstorder.
 Qed.
 
-Lemma pimpl_or_r: forall (a b c: @pred len V),
+Lemma pimpl_or_r: forall (a b c: @pred AT AEQ V),
   ((a =p=> b) \/ (a =p=> c))
   -> (a =p=> b \/ c).
 Proof.
@@ -733,28 +735,28 @@ Proof.
 Qed.
 
 Lemma pimpl_any :
-  forall (p : @pred len V),
+  forall (p : @pred AT AEQ V),
   p =p=> any.
 Proof.
   firstorder.
 Qed.
 
 Lemma pimpl_emp_any :
-  forall (p : @pred len V),
+  forall (p : @pred AT AEQ V),
   p =p=> emp * any.
 Proof.
   intros.
   eapply pimpl_trans; [|apply pimpl_star_emp]; apply pimpl_any.
 Qed.
 
-Lemma eq_pimpl : forall (a b : @pred len V),
+Lemma eq_pimpl : forall (a b : @pred AT AEQ V),
   a = b
   -> (a =p=> b).
 Proof.
   intros; subst; firstorder.
 Qed.
 
-Theorem sep_star_indomain : forall (p q : @pred len V) a,
+Theorem sep_star_indomain : forall (p q : @pred AT AEQ V) a,
   (p =p=> indomain a) ->
   (p * q =p=> indomain a).
 Proof.
@@ -766,13 +768,13 @@ Proof.
   eauto.
 Qed.
 
-Theorem ptsto_indomain : forall (a : word len) (v : V),
-  a |-> v =p=> indomain a.
+Theorem ptsto_indomain : forall (a : AT) (v : V),
+  a |-> v =p=> (@indomain AT AEQ V) a.
 Proof.
   firstorder.
 Qed.
 
-Theorem sep_star_ptsto_some : forall (a : word len) (v : V) F m,
+Theorem sep_star_ptsto_some : forall a v F (m : @mem AT AEQ V),
   (a |-> v * F)%pred m -> m a = Some v.
 Proof.
   unfold_sep_star; unfold ptsto, mem_union, exis.
@@ -782,7 +784,7 @@ Proof.
   auto.
 Qed.
 
-Theorem sep_star_ptsto_indomain : forall (a : word len) (v : V) F m,
+Theorem sep_star_ptsto_indomain : forall a v F (m : @mem AT AEQ V),
   (a |-> v * F)%pred m -> indomain a m.
 Proof.
   intros.
@@ -792,7 +794,7 @@ Qed.
 
 Definition pair_args_helper (A B C:Type) (f: A->B->C) (x: A*B) := f (fst x) (snd x).
 
-Theorem sep_star_or_distr : forall (a b c : @pred len V),
+Theorem sep_star_or_distr : forall (a b c : @pred AT AEQ V),
   (a * (b \/ c))%pred <=p=> (a * b \/ a * c)%pred.
 Proof.
   split.
@@ -807,33 +809,33 @@ Proof.
       apply pimpl_or_r; right; apply pimpl_refl.
 Qed.
 
-Theorem lift_impl : forall (P : @pred len V) (Q : Prop), (forall m, P m -> Q) -> P =p=> [[ Q ]] * P.
+Theorem lift_impl : forall (P : @pred AT AEQ V) (Q : Prop), (forall m, P m -> Q) -> P =p=> [[ Q ]] * P.
 Proof.
   intros. unfold_sep_star.
   exists (fun _ => None). exists m.
   intuition; hnf; try tauto; firstorder discriminate.
 Qed.
 
-Theorem ptsto_complete : forall (a : word len) (v : V) m1 m2,
+Theorem ptsto_complete : forall a v (m1 m2 : @mem AT AEQ V),
   (a |-> v)%pred m1 -> (a |-> v)%pred m2 -> m1 = m2.
 Proof.
   unfold ptsto; intros; apply functional_extensionality; intros.
   destruct H; destruct H0.
-  destruct (weq a x); subst; try congruence.
+  destruct (AEQ a x); subst; try congruence.
   erewrite H1; eauto.
   erewrite H2; eauto.
 Qed.
 
 Theorem emp_complete : forall m1 m2,
-  (@emp len V) m1 -> emp m2 -> m1 = m2.
+  (@emp AT AEQ V) m1 -> emp m2 -> m1 = m2.
 Proof.
   intros.
   apply functional_extensionality; unfold emp in *; congruence.
 Qed.
 
-Definition empty_mem {len : nat} {V : Type} : @mem len V := fun a => None.
+Definition empty_mem {AT : Type} {AEQ : DecEq AT} {V : Type} : @mem AT AEQ V := fun a => None.
 
-Theorem sep_star_empty_mem : forall (a b : @pred len V),
+Theorem sep_star_empty_mem : forall (a b : @pred AT AEQ V),
   (a * b)%pred empty_mem -> a empty_mem /\ b empty_mem.
 Proof.
   unfold_sep_star.
@@ -856,8 +858,8 @@ Proof.
   destruct (x fa); auto.
 Qed.
 
-Theorem ptsto_empty_mem : forall (a : word len) (v : V),
-  ~ (a |-> v)%pred empty_mem.
+Theorem ptsto_empty_mem : forall a v,
+  ~ (a |-> v)%pred (@empty_mem AT AEQ V).
 Proof.
   unfold empty_mem, ptsto.
   intuition discriminate.
@@ -866,43 +868,43 @@ Qed.
 End GenPredThm.
 
 
-Instance piff_equiv {len V} :
-  Equivalence (@piff len V).
+Instance piff_equiv {AT AEQ V} :
+  Equivalence (@piff AT AEQ V).
 Proof.
   split.
-  exact (@piff_refl len V).
-  exact (@piff_comm len V).
-  exact (@piff_trans len V).
+  exact (@piff_refl AT AEQ V).
+  exact (@piff_comm AT AEQ V).
+  exact (@piff_trans AT AEQ V).
 Qed.
 
-Instance pimpl_preorder {len V} :
-  PreOrder (@pimpl len V).
+Instance pimpl_preorder {AT AEQ V} :
+  PreOrder (@pimpl AT AEQ V).
 Proof.
   split.
-  exact (@pimpl_refl len V).
-  exact (@pimpl_trans len V).
+  exact (@pimpl_refl AT AEQ V).
+  exact (@pimpl_trans AT AEQ V).
 Qed.
 
-Instance pimpl_piff_proper {len V} :
-  Proper (piff ==> piff ==> Basics.flip Basics.impl) (@pimpl len V).
+Instance pimpl_piff_proper {AT AEQ V} :
+  Proper (piff ==> piff ==> Basics.flip Basics.impl) (@pimpl AT AEQ V).
 Proof.
   firstorder.
 Qed.
 
-Instance pimpl_pimpl_proper1 {len V} :
-  Proper (pimpl ==> Basics.flip pimpl ==> Basics.flip Basics.impl) (@pimpl len V).
+Instance pimpl_pimpl_proper1 {AT AEQ V} :
+  Proper (pimpl ==> Basics.flip pimpl ==> Basics.flip Basics.impl) (@pimpl AT AEQ V).
 Proof.
   firstorder.
 Qed.
 
-Instance pimpl_pimpl_proper2 {len V} :
-  Proper (Basics.flip pimpl ==> pimpl ==> Basics.impl) (@pimpl len V).
+Instance pimpl_pimpl_proper2 {AT AEQ V} :
+  Proper (Basics.flip pimpl ==> pimpl ==> Basics.impl) (@pimpl AT AEQ V).
 Proof.
   firstorder.
 Qed.
 
-Instance sep_star_apply_pimpl_proper {len V} :
-  Proper (pimpl ==> pimpl ==> eq ==> Basics.impl) (@sep_star len V).
+Instance sep_star_apply_pimpl_proper {AT AEQ V} :
+  Proper (pimpl ==> pimpl ==> eq ==> Basics.impl) (@sep_star AT AEQ V).
 Proof.
   intros p p' Hp q q' Hq m m' Hm H.
   subst.
@@ -911,8 +913,8 @@ Proof.
 Qed.
 
 
-Instance sep_star_apply_piff_proper {len V} :
-  Proper (piff ==> piff ==> eq ==> Basics.impl) (@sep_star len V).
+Instance sep_star_apply_piff_proper {AT AEQ V} :
+  Proper (piff ==> piff ==> eq ==> Basics.impl) (@sep_star AT AEQ V).
 Proof.
   intros p p' Hp q q' Hq m m' Hm H.
   subst.
@@ -923,45 +925,45 @@ Proof.
 Qed.
 
 
-Instance sep_star_piff_proper {len V} :
-  Proper (piff ==> piff ==> piff) (@sep_star len V).
+Instance sep_star_piff_proper {AT AEQ V} :
+  Proper (piff ==> piff ==> piff) (@sep_star AT AEQ V).
 Proof.
   intros a b H c d H'.
   split; ( apply pimpl_sep_star; [ apply H | apply H' ] ).
 Qed.
 
-Instance sep_star_pimpl_proper {len V} :
-  Proper (pimpl ==> pimpl ==> pimpl) (@sep_star len V).
+Instance sep_star_pimpl_proper {AT AEQ V} :
+  Proper (pimpl ==> pimpl ==> pimpl) (@sep_star AT AEQ V).
 Proof.
   intros a b H c d H'.
   apply pimpl_sep_star; assumption.
 Qed.
 
-Instance and_piff_proper {len V} :
-  Proper (piff ==> piff ==> piff) (@and len V).
+Instance and_piff_proper {AT AEQ V} :
+  Proper (piff ==> piff ==> piff) (@and AT AEQ V).
 Proof.
   firstorder.
 Qed.
 
-Instance and_pimpl_proper {len V} :
-  Proper (pimpl ==> pimpl ==> pimpl) (@and len V).
+Instance and_pimpl_proper {AT AEQ V} :
+  Proper (pimpl ==> pimpl ==> pimpl) (@and AT AEQ V).
 Proof.
   firstorder.
 Qed.
 
-Instance or_piff_proper {len V} :
-  Proper (piff ==> piff ==> piff) (@or len V).
+Instance or_piff_proper {AT AEQ V} :
+  Proper (piff ==> piff ==> piff) (@or AT AEQ V).
 Proof.
   firstorder.
 Qed.
 
-Instance or_pimpl_proper {len V} :
-  Proper (pimpl ==> pimpl ==> pimpl) (@or len V).
+Instance or_pimpl_proper {AT AEQ V} :
+  Proper (pimpl ==> pimpl ==> pimpl) (@or AT AEQ V).
 Proof.
   firstorder.
 Qed.
 
-Example pimpl_rewrite : forall len V a b (p : @pred len V) q x y, p =p=> q
+Example pimpl_rewrite : forall AT AEQ V a b (p : @pred AT AEQ V) q x y, p =p=> q
   -> (x /\ a * p * b \/ y =p=> x /\ a * q * b \/ y).
 Proof.
   intros.
@@ -969,13 +971,13 @@ Proof.
   reflexivity.
 Qed.
 
-Instance exists_proper {len V} {A : Type} :
-  Proper (pointwise_relation A pimpl ==> pimpl) (@exis len V A).
+Instance exists_proper {AT AEQ V} {A : Type} :
+  Proper (pointwise_relation A pimpl ==> pimpl) (@exis AT AEQ V A).
 Proof.
   firstorder.
 Qed.
 
-Example pimpl_exists_rewrite : forall len V (p : @pred len V) q, p =p=> q
+Example pimpl_exists_rewrite : forall AT AEQ V (p : @pred AT AEQ V) q, p =p=> q
   -> (exists x, p * x) =p=> (exists x, q * x).
 Proof.
   intros.
@@ -988,8 +990,8 @@ Qed.
  * an [exis] is applied to a [mem], and [setoid_rewrite] tries to rewrite the
  * term that appears under [exis].
  *)
-Instance exists_proper_impl {len V} {A : Type} :
-  Proper (pointwise_relation A piff ==> eq ==> iff) (@exis len V A).
+Instance exists_proper_impl {AT AEQ V} {A : Type} :
+  Proper (pointwise_relation A piff ==> eq ==> iff) (@exis AT AEQ V A).
 Proof.
   intros a b Hab m1 m2 Hm.
   split; unfold Basics.impl, exis; intros; deex; eexists.
@@ -1001,8 +1003,8 @@ Qed.
  * The following instance is needed to make [setoid_rewrite] fast on terms
  * that involve [lift_empty].  Otherwise, typeclass search takes forever.
  *)
-Instance lift_empty_proper {len V} :
-  Proper (iff ==> @piff _ _) (@lift_empty len V).
+Instance lift_empty_proper {AT AEQ V} :
+  Proper (iff ==> @piff _ _ _) (@lift_empty AT AEQ V).
 Proof.
   firstorder.
 Qed.
@@ -1010,14 +1012,14 @@ Qed.
 
 (* Specialized relations for [@pred valuset], to deal with async IO *)
 
-Theorem crash_xform_apply : forall (p : @pred addrlen valuset) (m m' : mem), possible_crash m m'
+Theorem crash_xform_apply : forall AT AEQ (p : @pred AT AEQ valuset) (m m' : @mem AT AEQ valuset), possible_crash m m'
   -> p m
   -> crash_xform p m'.
 Proof.
   unfold crash_xform; eauto.
 Qed.
 
-Theorem possible_crash_mem_union : forall (ma mb m' : mem), possible_crash (mem_union ma mb) m'
+Theorem possible_crash_mem_union : forall AT AEQ (ma mb m' : @mem AT AEQ _), possible_crash (mem_union ma mb) m'
   -> mem_disjoint ma mb
   -> exists ma' mb', m' = mem_union ma' mb' /\ mem_disjoint ma' mb' /\
                      possible_crash ma ma' /\ possible_crash mb mb'.
@@ -1055,7 +1057,7 @@ Proof.
     congruence.
 Qed.
 
-Theorem possible_crash_disjoint : forall ma mb ma' mb', mem_disjoint ma' mb'
+Theorem possible_crash_disjoint : forall AT AEQ (ma mb ma' mb' : @mem AT AEQ _), mem_disjoint ma' mb'
   -> possible_crash ma ma'
   -> possible_crash mb mb'
   -> mem_disjoint ma mb.
@@ -1069,7 +1071,7 @@ Proof.
   do 3 eexists; eauto.
 Qed.
 
-Theorem possible_crash_union : forall ma mb ma' mb', possible_crash ma ma'
+Theorem possible_crash_union : forall AT AEQ (ma mb ma' mb' : @mem AT AEQ _), possible_crash ma ma'
   -> possible_crash mb mb'
   -> possible_crash (mem_union ma mb) (mem_union ma' mb').
 Proof.
@@ -1089,7 +1091,7 @@ Proof.
     right. do 2 eexists. intuition.
 Qed.
 
-Theorem possible_crash_trans : forall ma mb mc,
+Theorem possible_crash_trans : forall AT AEQ (ma mb mc : @mem AT AEQ _),
   possible_crash ma mb ->
   possible_crash mb mc ->
   possible_crash ma mc.
@@ -1106,14 +1108,14 @@ Proof.
   inversion H1.
 Qed.
 
-Theorem crash_xform_idem : forall p, crash_xform (crash_xform p) =p=> crash_xform p.
+Theorem crash_xform_idem : forall AT AEQ (p : @pred AT AEQ _), crash_xform (crash_xform p) =p=> crash_xform p.
 Proof.
   unfold crash_xform, pimpl; intros.
   repeat deex; eexists; intuition eauto.
   eapply possible_crash_trans; eauto.
 Qed.
 
-Theorem crash_xform_sep_star_dist : forall (p q : pred),
+Theorem crash_xform_sep_star_dist : forall AT AEQ (p q : @pred AT AEQ _),
   crash_xform (p * q) <=p=> crash_xform p * crash_xform q.
 Proof.
   unfold_sep_star; unfold crash_xform, piff, pimpl; split; intros; repeat deex.
@@ -1125,14 +1127,14 @@ Proof.
     apply possible_crash_union; eauto.
 Qed.
 
-Theorem crash_xform_or_dist : forall (p q : pred),
+Theorem crash_xform_or_dist : forall AT AEQ (p q : @pred AT AEQ _),
   crash_xform (p \/ q) <=p=> crash_xform p \/ crash_xform q.
 Proof.
   firstorder.
 Qed.
 
-Theorem crash_xform_lift_empty : forall (P : Prop),
-  crash_xform [[ P ]] <=p=> [[ P ]].
+Theorem crash_xform_lift_empty : forall AT AEQ (P : Prop),
+  @crash_xform AT AEQ [[ P ]] <=p=> [[ P ]].
 Proof.
   unfold crash_xform, lift_empty, possible_crash; intros; split;
     intros m H; repeat deex.
@@ -1141,7 +1143,7 @@ Proof.
   eexists; intuition.
 Qed.
 
-Theorem crash_xform_sep_star_apply : forall (p q : pred) (m m' : mem), possible_crash m m'
+Theorem crash_xform_sep_star_apply : forall AT AEQ (p q : @pred AT AEQ _) (m m' : mem), possible_crash m m'
   -> (p * q)%pred m
   -> (crash_xform p * crash_xform q)%pred m'.
 Proof.
@@ -1150,29 +1152,29 @@ Proof.
   do 2 eexists; repeat split; auto; unfold crash_xform; eexists; split; eauto.
 Qed.
 
-Theorem crash_xform_exists_comm : forall T (p : T -> pred),
+Theorem crash_xform_exists_comm : forall AT AEQ T (p : T -> @pred AT AEQ _),
   crash_xform (exists x, p x) =p=> exists x, crash_xform (p x).
 Proof.
   unfold crash_xform, exis, pimpl; intros.
   repeat deex; repeat eexists; intuition eauto.
 Qed.
 
-Theorem crash_xform_pimpl : forall p q, p =p=>q
+Theorem crash_xform_pimpl : forall AT AEQ (p q : @pred AT AEQ _), p =p=>q
   -> crash_xform p =p=> crash_xform q.
 Proof.
   unfold crash_xform, pimpl; intros.
   repeat deex; eexists; intuition eauto.
 Qed.
 
-Instance crash_xform_pimpl_proper :
-  Proper (pimpl ==> pimpl) crash_xform.
+Instance crash_xform_pimpl_proper {AT AEQ} :
+  Proper (pimpl ==> pimpl) (@crash_xform AT AEQ).
 Proof.
   intros p q Hp.
   apply crash_xform_pimpl; auto.
 Qed.
 
-Theorem crash_invariant_ptsto: forall a v,
-  crash_xform (a |=> v) =p=> a |=> v.
+Theorem crash_invariant_ptsto: forall AT AEQ a v,
+  (@crash_xform AT AEQ) (a |=> v) =p=> a |=> v.
 Proof.
   unfold crash_xform, pimpl, possible_crash, ptsto; intros.
   deex; intuition eauto.
@@ -1188,7 +1190,7 @@ Proof.
 Qed.
 
 Lemma ptsto_synced_valid:
-  forall len (a : word len) v F m,
+  forall AT AEQ a v F (m : @mem AT AEQ _),
   (a |=> v * F)%pred m
   -> m a = Some (v, nil).
 Proof.
@@ -1197,7 +1199,7 @@ Proof.
 Qed.
 
 Lemma ptsto_cur_valid:
-  forall len (a : word len) v F m,
+  forall AT AEQ a v F (m : @mem AT AEQ _),
   (a |~> v * F)%pred m
   -> exists l, m a = Some (v, l).
 Proof.
