src/ListPred.v
@@ -10,9 +10,10 @@ A general list predicate *)
 Section LISTPRED.
 
   Variable T : Type.
-  Variable len : nat.
+  Variable AT : Type.
+  Variable AEQ : DecEq AT.
   Variable V : Type.
-  Variable prd : T -> @pred len V.
+  Variable prd : T -> @pred AT AEQ V.
 
   Fixpoint listpred (ts : list T) :=
     match ts with
@@ -20,7 +21,7 @@ Section LISTPRED.
     | t :: ts' => (prd t) * listpred ts'
     end%pred.
 
-  Lemma listpred_nil: forall T len V (prd : T -> @pred len V),
+  Lemma listpred_nil:
     listpred nil = emp.
   Proof.
     unfold listpred; intros; auto.
@@ -61,7 +62,7 @@ Section LISTPRED.
      intros; subst; auto.
   Qed.
 
-  Definition sep_star_fold : (T -> @pred len V -> @pred len V) := fun x => sep_star (prd x).
+  Definition sep_star_fold : (T -> @pred AT AEQ V -> @pred AT AEQ V) := fun x => sep_star (prd x).
   Definition listpred' := fold_right sep_star_fold emp.
 
   Theorem listpred_listpred': forall l,
@@ -158,9 +159,10 @@ Section LISTMATCH.
 
   Variable A : Type.
   Variable B : Type.
-  Variable len : nat.
+  Variable AT : Type.
+  Variable AEQ : DecEq AT.
   Variable V : Type.
-  Variable prd : A -> B -> @pred len V.
+  Variable prd : A -> B -> @pred AT AEQ V.
 
   Definition pprd := prod_curry prd.
 
